Added remaining morph lemmas

examples/refinement/generic/Eq.fst
@@ -93,7 +93,7 @@ let morph_return' #lstate (#lw:low_state lstate) #hstate (#p: state_lens lstate 
 
 (* This formulation does not seem provable *)
 [@expect_failure]
-let morph_return #lstate (#lw:low_state lstate) #hstate (#p: state_lens lstate hstate) #a
+let morph_return_fail #lstate (#lw:low_state lstate) #hstate (#p: state_lens lstate hstate) #a
   (wp : hwp_mon #hstate a) (c:high a wp) (x:a) :
   Lemma
     (requires (implies wp (return_wp x) /\ c == return_elab x))
@@ -104,17 +104,17 @@ let morph_return #lstate (#lw:low_state lstate) #hstate (#p: state_lens lstate h
   assert (c == cast #hstate #a #_ wp #i' (return_elab x));
   ()
 
-(* We would have to write something like this instead *)
-let morph_return'' #lstate (#lw:low_state lstate) #hstate (#p: state_lens lstate hstate) #a
-    (wp : hwp_mon #hstate a) (c:high a wp) (x:a) :
-  Lemma
-    (requires (implies wp (return_wp x) /\ c == return_elab x))
-    (ensures (l_eq wp c (morph #_ #lw  #_ #p a wp c) 
-                   wp (return_elab x) (lcast (return_wp x) wp (return_elab x) (lreturn x)))) =
-  ()
+// (* We would have to write something like this instead *)
+// Redundant 
+// let morph_return'' #lstate (#lw:low_state lstate) #hstate (#p: state_lens lstate hstate) #a
+//     (wp : hwp_mon #hstate a) (c:high a wp) (x:a) :
+//   Lemma
+//     (requires (implies wp (return_wp x) /\ c == return_elab x))
+//     (ensures (l_eq wp c (morph #_ #lw  #_ #p a wp c) 
+//                    wp (return_elab x) (lcast (return_wp x) wp (return_elab x) (lreturn x)))) =
+//   ()
 
-(* or even better *)
-let morph_return''' #lstate (#lw:low_state lstate) #hstate (#p: state_lens lstate hstate) #a
+let morph_return #lstate (#lw:low_state lstate) #hstate (#p: state_lens lstate hstate) #a
     (wp : hwp_mon #hstate a) (c:high a wp) (x:a) :
   Lemma
     (requires (implies wp (return_wp x) /\ c == return_elab x))
@@ -123,7 +123,7 @@ let morph_return''' #lstate (#lw:low_state lstate) #hstate (#p: state_lens lstat
   ()
 
 
-let morph_bind''' #lstate (lw:low_state lstate) #hstate (#p: state_lens lstate hstate) #a #b
+let morph_bind #lstate (lw:low_state lstate) #hstate (#p: state_lens lstate hstate) #a #b
     (wp : hwp_mon #hstate b) (c:high b wp)
     (wp1 : hwp_mon #hstate a) (c1:high a wp1)
     (fwp : a -> hwp_mon #hstate b) (fc:(x:a) -> high b (fwp x))
@@ -132,5 +132,56 @@ let morph_bind''' #lstate (lw:low_state lstate) #hstate (#p: state_lens lstate h
     (requires (implies wp (bind_wp wp1 fwp) /\ c == bind_elab c1 fc))
     (ensures (l_eq wp c (morph #_ #lw  #_ #p b wp c) 
                    wp (bind_elab c1 fc) (lbind #_ #lw #_ #p (morph #_ #lw #_ #p a wp1 c1) (fun x -> morph #_ #lw #_ #p b (fwp x) (fc x))))) =
+  ()
+
+let morph_write lstate (lw:low_state lstate) #hstate (#p: state_lens lstate hstate)
+    (wp : hwp_mon #hstate unit) (c:high unit wp) (s:hstate) :
+  Lemma
+    (requires (implies wp (write_wp s) /\ c == write_elab s))
+    (ensures (l_eq wp c (morph #_ #lw  #_ #p unit wp c) 
+                   wp (write_elab s) (lwrite #_ #lw #_ #p s))) =
+   ()
+
+let morph_read lstate (lw:low_state lstate) #hstate (#p: state_lens lstate hstate)
+    (wp : hwp_mon #hstate hstate) (c:high hstate wp) :
+  Lemma
+    (requires (implies wp read_wp) /\ c == read_elab ())
+    (ensures (l_eq wp c (morph #_ #lw  #_ #p hstate wp c) 
+                   wp (read_elab ()) (lread #_ #lw #_ #p ()))) =
+  ()
+
+let morph_write_comp lstate (lw:low_state lstate) #hstate (#p: state_lens lstate hstate)
+    (#a:Type) (#l1:lens hstate a) (l2:state_lens lstate a) (#cm:commutes p l1 l2)
+    (wp : hwp_mon #hstate unit) (c:high unit wp) (x:a) :
+  Lemma
+    (requires (implies wp (write_comp_wp l1 x) /\ c == write_comp l1 x))
+    (ensures (l_eq wp c (morph #_ #lw  #_ #p unit wp c) 
+                   wp (write_comp l1 x) (lwrite_comp #_ #lw #_ #p #a #l1 l2 #cm x))) =
+  ()
+
+let morph_read_comp lstate (lw:low_state lstate) #hstate (#p: state_lens lstate hstate)
+    (#a:Type) (#l1:lens hstate a) (l2:state_lens lstate a) (#cm:commutes p l1 l2)
+    (wp : hwp_mon #hstate a) (c:high a wp) :
+  Lemma
+    (requires (implies wp (read_comp_wp l1)) /\ c == read_comp l1 ())
+    (ensures (l_eq wp c (morph #_ #lw  #_ #p a wp c) 
+                   wp (read_comp l1 ()) (lread_comp #_ #lw #_ #p #a #l1 l2 #cm ()))) =
+  ()
+
+unfold
+let inv_as_wp (#state : Type) (#a : Type) (inv : state -> int -> Type0) lo hi
+: hwp_mon #state a =
+  as_wp (fun h0 -> inv h0 lo) (fun h0 _ h1 -> inv h1 hi)
+
+let morph_for lstate (lw:low_state lstate) #hstate (#p: state_lens lstate hstate)
+    (wp : hwp_mon #hstate unit) (c:high unit wp)
+    (inv : hstate -> int -> Type0)
+    (f : (i:int) -> high_p unit (requires (fun h0 -> inv h0 i))
+                             (ensures (fun h0 _ h1 -> inv h1 (i + 1)))) 
+    (lo : int) (hi : int{lo <= hi}) :
+  Lemma 
+    (requires ((implies wp (inv_as_wp inv lo hi)) /\ c == for_elab inv f lo hi))
+    (ensures (l_eq wp c (morph #_ #lw  #_ #p unit wp c) 
+                   wp (for_elab inv f lo hi) (lfor' #_ #lw #_ #p inv f (fun i -> morph #_ #lw #_ #p unit _ (f i)) lo hi))) = 
   ()
 
